hol/p4_exec_sem_stmt_soundnessScript.sml
@@ -92,15 +92,92 @@ Theorem stmt_trans_exec_sound_red:
  e_exec_sound e ==>
  stmt_exec_sound (stmt_trans e)
 Proof
-cheat
+fs [stmt_exec_sound, e_exec_sound] >>
+rpt strip_tac >>
+Cases_on `status` >> (
+ fs [stmt_exec]
+) >>
+Cases_on `is_v e` >> (
+ fs []
+) >| [
+ Cases_on `e` >> (
+  fs [is_v]
+ ) >>
+ Cases_on `v` >> (
+  fs [is_v_str]
+ ) >>
+ rw [] >>
+ fs [stmt_exec_trans] >>
+ METIS_TAC [(valOf o find_clause_stmt_red) "stmt_trans", clause_name_def],
+
+ Cases_on `e_exec ctx g_scope_list scopes_stack e` >> (
+  fs []
+ ) >>
+ pairLib.PairCases_on `x` >>
+ fs [] >>
+ METIS_TAC [(valOf o find_clause_stmt_red) "stmt_trans_e", clause_name_def]
+]
 QED
 
-Theorem stmt_block_exec_sound_red:
-!stmt decl_list.
-stmt_exec_sound stmt ==>
-stmt_exec_sound (stmt_block decl_list stmt)
+Theorem stmt_app_exec_sound_red:
+!e_l tbl.
+ (!e. e_exec_sound e) ==>
+(* OR: l_sound e_l ==> ? *)
+ stmt_exec_sound (stmt_app tbl e_l)
 Proof
-cheat
+fs [stmt_exec_sound] >>
+rpt strip_tac >>
+pairLib.PairCases_on `ctx` >>
+rename1 `(ctx0, func_map, b_func_map, pars_map, tbl_map)` >>
+rename1 `(ext_map, func_map, b_func_map, pars_map, tbl_map)` >>
+Cases_on `status` >> (
+ fs [stmt_exec]
+) >>
+Cases_on `index_not_const e_l` >> (
+ fs []
+) >| [
+ (* TODO: stmt_apply_table_v *)
+ Cases_on `FLOOKUP tbl_map tbl` >> (
+  fs []
+ ) >>
+ Cases_on `ctrl (tbl,e_l,x)` >> (
+  fs []
+ ) >>
+ pairLib.PairCases_on `x'` >>
+ fs [] >>
+ rw [] >>
+ cheat,
+
+ (* TODO: stmt_apply_table_e *)
+ cheat
+]
+(* OLD:
+Cases_on `get_v e` >> (
+ fs []
+) >| [
+ Cases_on `e_exec (ext_map, func_map, tbl_map) g_scope_list scopes_stack e` >> (
+  fs []
+ ) >>
+ pairLib.PairCases_on `x` >>
+ fs [] >>
+ METIS_TAC [(valOf o find_clause_stmt_red) "stmt_apply_table_e", clause_name_def],
+
+ Cases_on `FLOOKUP tbl_map s` >> (
+  fs []
+ ) >>
+ pairLib.PairCases_on `x'` >>
+ fs [] >>
+ Cases_on `ctrl (s,x,x'1)` >> (
+  fs []
+ ) >>
+ pairLib.PairCases_on `x'` >>
+ fs [] >>
+ Cases_on `e` >> (
+  fs [get_v]
+ ) >>
+ METIS_TAC [(valOf o find_clause_stmt_red) "stmt_apply_table_v", clause_name_def]
+]
+*)
 QED
 
 Theorem stmt_verify_exec_sound_red:
@@ -184,50 +261,332 @@ Cases_on `is_v e1` >> Cases_on `is_v e2` >| [
 ]
 QED
 
+Theorem stmt_ass_exec_sound_red:
+!lval e.
+e_exec_sound e ==>
+stmt_exec_sound (stmt_ass lval e)
+Proof
+fs [stmt_exec_sound, e_exec_sound] >>
+rpt strip_tac >>
+Cases_on `status` >> (
+ fs [stmt_exec]
+) >>
+Cases_on `is_v e` >> (
+ fs []
+) >| [
+ Cases_on `stmt_exec_ass lval e (g_scope_list ++ scopes_stack)` >> (
+  fs []
+ ) >>
+ Cases_on `e` >> (
+  fs [is_v]
+ ) >>
+ rename1 `TAKE 2 g_scope_list'` >>
+ rw [] >>
+ fs [stmt_exec_ass] >>
+ subgoal `?g_scope g_scope'. TAKE 2 g_scope_list' = [g_scope; g_scope']` >- (
+  cheat
+ ) >>
+ subgoal `?scopes_stack''. DROP 2 g_scope_list' = scopes_stack''` >- (
+  cheat
+ ) >>
+ fs [] >>
+ irule ((valOf o find_clause_stmt_red) "stmt_ass_v") >>
+ fs [clause_name_def] >>
+ rpt conj_tac >| [
+  Cases_on `g_scope_list'` >> (
+   fs []
+  ),
+
+  Cases_on `g_scope_list'` >> (
+   fs []
+  ) >>
+  Cases_on `t` >> (
+   fs []
+  ),
+
+  Cases_on `g_scope_list'` >> (
+   fs []
+  ) >>
+  Cases_on `t` >> (
+   fs []
+  )
+ ],
+
+ Cases_on `e_exec ctx g_scope_list scopes_stack e` >> (
+  fs []
+ ) >>
+ pairLib.PairCases_on `x` >>
+ fs [] >>
+ METIS_TAC [((valOf o find_clause_stmt_red) "stmt_ass_e"), clause_name_def]
+]
+QED
+
+Theorem stmt_seq_exec_sound_red:
+!s1 s2.
+stmt_exec_sound s1 ==>
+stmt_exec_sound s2 ==>
+stmt_exec_sound (stmt_seq s1 s2)
+Proof
+fs [stmt_exec_sound] >>
+rpt strip_tac >>
+Cases_on `status` >> (
+ fs [stmt_exec]
+) >>
+Cases_on `is_empty s1` >> (
+ fs []
+) >| [
+ Cases_on `s1` >> (
+  fs [is_empty]
+ ) >>
+ METIS_TAC [((valOf o find_clause_stmt_red) "stmt_seq2"), clause_name_def],
+
+ Cases_on `stmt_exec ctx (g_scope_list,[(funn,[s1],scopes_stack)],ctrl,status_running)` >> (
+  fs []
+ ) >>
+ pairLib.PairCases_on `x` >> (
+  fs []
+ ) >>
+ Cases_on `x1` >> (
+  fs []
+ ) >>
+ Cases_on `t` >> (
+  fs []
+ ) >| [
+  pairLib.PairCases_on `h` >> (
+   fs []
+  ) >>
+  Cases_on `h1` >> (
+   fs []
+  ) >>
+  Cases_on `t` >> (
+   fs []
+  ) >| [
+   Cases_on `x3` >> (
+    fs []
+   ) >| [
+    rw [] >>
+    rename1 `(x0, [(funn', [stmt_seq s1' s2], scopes_stack')], ctrl', status_running)` >>
+    rename1 `(g_scope_list', [(funn', [stmt_seq s1' s2], scopes_stack')], ctrl', status_running)` >>
+    (* TODO *)
+    Q.SUBGOAL_THEN `funn' = funn`
+     (fn thm => fs [thm]) >- (
+     cheat
+    ) >>
+    Q.SUBGOAL_THEN `[(funn, [stmt_seq s1' s2], scopes_stack')] = [] ++ [(funn, [stmt_seq s1' s2], scopes_stack')]`
+     (fn thm => ONCE_REWRITE_TAC [thm]) >- (
+     fs []
+    ) >>
+    Q.SUBGOAL_THEN `[(funn, [stmt_seq s1' s2], scopes_stack')] = [(funn, [] ++ [stmt_seq s1' s2], scopes_stack')]`
+     (fn thm => ONCE_REWRITE_TAC [thm]) >- (
+     fs []
+    ) >>
+    irule ((valOf o find_clause_stmt_red) "stmt_seq1") >>
+    fs [clause_name_def],
+
+    rw [] >>
+    rename1 `(x0, [(funn', [s], scopes_stack')], ctrl', status_returnv v)` >>
+    rename1 `(g_scope_list', [(funn', [s], scopes_stack')], ctrl', status_returnv v)` >>
+    (* TODO *)
+    Q.SUBGOAL_THEN `funn' = funn`
+     (fn thm => fs [thm]) >- (
+     cheat
+    ) >>
+    METIS_TAC [((valOf o find_clause_stmt_red) "stmt_seq3"), clause_name_def, status_distinct],
+
+    rw [] >>
+    rename1 `(x0, [(funn', [s1'], scopes_stack')], ctrl', status_trans s)` >>
+    rename1 `(g_scope_list', [(funn', [s1'], scopes_stack')], ctrl', status_trans s)` >>
+    (* TODO *)
+    Q.SUBGOAL_THEN `funn' = funn`
+     (fn thm => fs [thm]) >- (
+     cheat
+    ) >>
+    METIS_TAC [((valOf o find_clause_stmt_red) "stmt_seq3"), clause_name_def, status_distinct],
+
+    rw [] >>
+    rename1 `(x0, [(funn', [s1'], scopes_stack')], ctrl', status_type_error)` >>
+    rename1 `(g_scope_list', [(funn', [s1'], scopes_stack')], ctrl', status_type_error)` >>
+    (* TODO *)
+    Q.SUBGOAL_THEN `funn' = funn`
+     (fn thm => fs [thm]) >- (
+     cheat
+    ) >>
+    METIS_TAC [((valOf o find_clause_stmt_red) "stmt_seq3"), clause_name_def, status_distinct]
+   ],
+
+   Cases_on `h'` >> (
+    fs []
+   ) >>
+   Cases_on `t'` >> (
+    fs []
+   ) >>
+   Cases_on `x3` >> (
+    fs []
+   ) >>
+   rw [] >>
+   (* TODO: seq1? *)
+   cheat
+  ],
+
+  pairLib.PairCases_on `h'` >> (
+   fs []
+  ) >>
+  Cases_on `h'1` >> (
+   fs []
+  ) >>
+  Cases_on `t` >> (
+   fs []
+  ) >>
+  Cases_on `t'` >> (
+   fs []
+  ) >>
+  Cases_on `x3` >> (
+   fs []
+  ) >>
+  (* TODO: seq1? *)
+  cheat
+ ]
+]
+(* OLD:
+ rename1 `(x0,frame_list',ctrl',status')` >>
+ rename1 `(g_scope_list',frame_list',ctrl',status')` >>
+ Cases_on `frame_list'` >> (
+  fs []
+ ) >>
+ Cases_on `t` >> (
+  fs []
+ ) >| [
+  pairLib.PairCases_on `h` >>
+  fs [] >>
+  rw [] >>
+  Cases_on `status'` >> (
+   fs []
+  ) >| [
+   Q.SUBGOAL_THEN `[(funn,stmt_seq h1 s2,h2)] = [] ++ [(funn,stmt_seq h1 s2,h2)]`
+    (fn thm => ONCE_REWRITE_TAC [thm]) >- (
+    fs []
+   ) >>
+   irule ((valOf o find_clause_stmt_red) "stmt_seq1") >>
+   fs [clause_name_def],
+
+   METIS_TAC [((valOf o find_clause_stmt_red) "stmt_seq3"), clause_name_def, status_distinct],
+
+   METIS_TAC [((valOf o find_clause_stmt_red) "stmt_seq3"), clause_name_def, status_distinct],
+
+   METIS_TAC [((valOf o find_clause_stmt_red) "stmt_seq3"), clause_name_def, status_distinct]
+  ],
+
+  pairLib.PairCases_on `h'` >>
+  fs [] >>
+  Cases_on `t'` >> (
+   fs []
+  ) >>
+  Cases_on `status'` >> (
+   fs []
+  ) >>
+  rw [] >>
+  Q.SUBGOAL_THEN `[h; (funn,stmt_seq h'1 s2,h'2)] = [h] ++ [(funn,stmt_seq h'1 s2,h'2)]`
+   (fn thm => ONCE_REWRITE_TAC [thm]) >- (
+   fs []
+  ) >>
+  irule ((valOf o find_clause_stmt_red) "stmt_seq1") >>
+  fs [clause_name_def]
+ ]
+]
+*)
+QED
+
+Theorem stmt_cond_exec_sound_red:
+!e s1 s2.
+e_exec_sound e ==>
+stmt_exec_sound s1 ==>
+stmt_exec_sound s2 ==>
+stmt_exec_sound (stmt_cond e s1 s2)
+Proof
+fs [stmt_exec_sound, e_exec_sound] >>
+rpt strip_tac >>
+Cases_on `status` >> (
+ fs [stmt_exec]
+) >>
+Cases_on `is_v_bool e` >> (
+ fs []
+) >| [
+ Cases_on `e` >> (
+  fs [is_v_bool]
+ ) >>
+ Cases_on `v` >> (
+  fs [is_v_bool]
+ ) >>
+ Cases_on `b` >> (
+  fs [stmt_exec_cond]
+ ) >| [
+  metis_tac [((valOf o find_clause_stmt_red) "stmt_cond2"), clause_name_def],
+
+  metis_tac [((valOf o find_clause_stmt_red) "stmt_cond3"), clause_name_def]
+ ],
+
+ Cases_on `e_exec ctx g_scope_list scopes_stack e` >> (
+  fs []
+ ) >>
+ pairLib.PairCases_on `x` >>
+ fs [] >>
+ metis_tac [((valOf o find_clause_stmt_red) "stmt_cond_e"), clause_name_def]
+]
+QED
+
+Theorem stmt_block_exec_sound_red:
+!s decl_list.
+stmt_exec_sound s ==>
+stmt_exec_sound (stmt_block decl_list s)
+Proof
+fs [stmt_exec_sound] >>
+rpt strip_tac >>
+Cases_on `status` >> (
+ fs [stmt_exec]
+) >>
+rw [] >>
+metis_tac [((valOf o find_clause_stmt_red) "stmt_block_enter"), clause_name_def]
+QED
+
 Theorem stmt_exec_sound_red:
 !stmt. stmt_exec_sound stmt
 Proof
 ASSUME_TAC e_exec_sound_red >>
 irule stmt_induction >>
-REPEAT STRIP_TAC >| [
+rpt strip_tac >| [
  (* Empty statement *)
  fs [stmt_exec_sound] >>
  rpt strip_tac >>
  Cases_on `status` >> (
   fs [stmt_exec]
  ) >>
- (* Block exit *)
+ (* TODO: Block exit? *)
  cheat,
 
  (* Extern *)
  fs [stmt_ext_exec_sound_red],
 
  (* Return statement *)
- (* TODO *)
- cheat,
+ fs [stmt_ret_exec_sound_red],
 
  (* Transition statement *)
- (* TODO *)
- cheat,
+ fs [stmt_trans_exec_sound_red],
 
  (* Verify statement *)
  fs [stmt_verify_exec_sound_red],
 
  (* Apply statement *)
- (* TODO *)
- cheat,
+ fs [stmt_app_exec_sound_red],
 
  (* Assign statement *)
  (* TODO *)
- cheat,
+ fs [stmt_ass_exec_sound_red],
 
  (* Sequence of statements *)
- (* TODO *)
- cheat,
+ fs [stmt_seq_exec_sound_red],
 
  (* Conditional statement *)
- (* TODO *)
- cheat,
+ fs [stmt_cond_exec_sound_red],
 
  (* Block entry *)
  fs [stmt_block_exec_sound_red]
